o Still working on abs2bot.

rules/proof.v
@@ -42,6 +42,7 @@ Require Export rules_function.
 
 Require Export computation10.
 Require Export computation_preserves_lib.
+Require Export computation_preserves_abs2bot.
 
 
 Inductive valid_rule {o} : @rule o -> Type :=
@@ -1063,25 +1064,6 @@ Fixpoint unfold_library {o} (l : library) (t : @NTerm o) : NTerm :=
     unfold_library entries (unfold_entry entry t)
   end.
 
-Definition abs2bot_op {o}
-           (op : @Opid o)
-           (bs : list BTerm) : NTerm :=
-  match op with
-  | Abs abs => mk_bot
-  | _ => oterm op bs
-  end.
-
-Fixpoint abs2bot {o} (t : @NTerm o) : NTerm :=
-  match t with
-  | vterm v => vterm v
-  | sterm f => sterm (fun n => abs2bot (f n))
-  | oterm op bs => abs2bot_op op (map abs2bot_bterm bs)
-  end
-with abs2bot_bterm {o} (b : @BTerm o) : BTerm :=
-       match b with
-       | bterm vs t => bterm vs (abs2bot t)
-       end.
-
 Definition unfold_lib {o} lib (t : @NTerm o) : NTerm :=
   abs2bot (unfold_library lib t).
 
@@ -1171,499 +1153,169 @@ Proof.
     introv; left; apply h.
 Qed.
 
-Lemma subset_nil_implies_nil :
-  forall T (l : list T), subset l [] -> l = [].
+Lemma reduces_to_abs2bot {o} :
+  forall (t : @NTerm o) u,
+    wf_term t
+    -> reduces_to [] t u
+    -> {w : NTerm
+        & reduces_to [] (abs2bot t) w
+        # alpha_eq w (abs2bot u)}.
 Proof.
-  introv ss.
-  destruct l as [|x l]; allsimpl; auto.
-  pose proof (ss x); allsimpl; tcsp.
-Qed.
-Hint Resolve subset_nil_implies_nil : slow.
+  introv wf comp.
+  allunfold @reduces_to; exrepnd.
+  revert dependent t.
+  induction k; introv wf comp.
 
-Lemma implies_props_abs2bot {o} :
-  forall (t : @NTerm o),
-    (nt_wf t -> nt_wf (abs2bot t))
-      # (subset (free_vars (abs2bot t)) (free_vars t))
-      # (subset (get_utokens (abs2bot t)) (get_utokens t)).
-Proof.
-  nterm_ind t as [v|f ind|op bs ind] Case; dands; introv h; allsimpl; auto.
-
-  - Case "sterm".
-    inversion h as [|? imp|]; subst.
-    constructor; introv.
-    pose proof (imp n) as q; clear imp; repnd.
-    pose proof (ind n) as z; clear ind; repnd.
-    apply z0 in q0.
-    rw q1 in z1.
-    rw q in z.
+  - allrw @reduces_in_atmost_k_steps_0; subst.
+    exists (abs2bot u).
     dands; auto.
+    exists 0.
+    apply reduces_in_atmost_k_steps_0; auto.
 
-    + unfold closed; eauto 3 with slow.
+  - rw @reduces_in_atmost_k_steps_S in comp; exrepnd.
+    pose proof (compute_step_abs2bot t u0 wf comp1) as h; exrepnd.
 
-    + unfold noutokens; eauto 3 with slow.
+    applydup @preserve_nt_wf_compute_step in comp1; eauto 3 with slow.
 
-  - Case "oterm".
-    unfold abs2bot_op.
-    inversion  h as [| |? ? imp e]; subst; clear h.
+    pose proof (IHk u0) as q; clear IHk.
+    repeat (autodimp q hyp); eauto 3 with slow.
+    exrepnd.
 
-    destruct op; allsimpl; eauto 2 with slow;
-    constructor; simpl; allrw map_map; allunfold @compose.
+    pose proof (reduces_in_atmost_k_steps_alpha [] (abs2bot u0) w) as q.
+    repeat (autodimp q hyp); eauto 3 with slow.
+    apply q in q2; clear q; exrepnd.
 
-    + introv i; allrw in_map_iff; exrepnd; subst.
-      destruct a as [l t]; simpl.
-      applydup ind in i1; repnd.
-      constructor.
-      apply i2.
-      apply imp in i1.
-      allrw @bt_wf_iff. auto.
-
-    + rw <- e.
-      apply eq_maps; introv i.
-      destruct x as [l t]; simpl; auto.
-
-    + introv i; allrw in_map_iff; exrepnd; subst.
-      destruct a as [l t]; simpl.
-      applydup ind in i1; repnd.
-      constructor.
-      apply i2.
-      apply imp in i1.
-      allrw @bt_wf_iff. auto.
-
-    + rw <- e.
-      apply eq_maps; introv i.
-      destruct x as [l t]; simpl; auto.
-
-    + introv i; allrw in_map_iff; exrepnd; subst.
-      destruct a as [l t]; simpl.
-      applydup ind in i1; repnd.
-      constructor.
-      apply i2.
-      apply imp in i1.
-      allrw @bt_wf_iff. auto.
-
-    + rw <- e.
-      apply eq_maps; introv i.
-      destruct x as [l t]; simpl; auto.
-
-  - Case "oterm".
-    destruct op; allsimpl; tcsp; allrw lin_flat_map; exrepnd;
-    allrw in_map_iff; exrepnd; subst;
-    destruct a as [l t]; allsimpl;
-    eexists; dands; eauto; allsimpl;
-    allrw in_remove_nvars; repnd; dands; auto;
-    apply ind in h1; repnd;
-    apply h4 in h2; auto.
-
-  - Case "oterm".
-    destruct op; allsimpl; tcsp; allrw in_app_iff; repndors; tcsp;
-    allrw lin_flat_map; exrepnd; try right;
-    destruct x0 as [l t]; allsimpl;
-    allrw in_map_iff; exrepnd;
-    destruct a as [l1 t1]; allsimpl; ginv;
-    applydup ind in h1; repnd;
+    exists t2'; dands; eauto 3 with slow.
+    exists (S k0).
+    rw @reduces_in_atmost_k_steps_S.
     eexists; dands; eauto.
 Qed.
 
-Lemma isprog_sterm_abs2bot {o} :
-  forall (f : @ntseq o),
-    isprog (sterm f)
-    -> isprog (sterm (fun n => abs2bot (f n))).
-Proof.
-  introv isp.
-  allrw @isprog_eq.
-  inversion isp as [cl wf].
-  rw @nt_wf_sterm_iff in wf.
-  apply nt_wf_sterm_implies_isprogram.
-  apply wfst; introv.
-  pose proof (wf n) as k; clear wf; repnd.
-  pose proof (implies_props_abs2bot (f n)) as h; repnd.
-  autodimp h0 hyp.
-  rw k1 in h1.
-  rw k in h.
-  apply subset_nil_implies_nil in h1.
-  apply subset_nil_implies_nil in h.
-  dands; auto.
-Qed.
-Hint Resolve isprog_sterm_abs2bot : slow.
-
-Lemma implies_isprog_abs2bot {o} :
+Lemma implies_isvalue_abs2bot {o} :
   forall (t : @NTerm o),
-    isprog t
-    -> isprog (abs2bot t).
+    isvalue t
+    -> isvalue (abs2bot t).
 Proof.
-  introv isp.
-  allrw @isprog_eq.
-  inversion isp as [cl wf].
-  pose proof (implies_props_abs2bot t) as h; repnd.
-  constructor; auto.
-  rw cl in h1.
-  apply subset_nil_implies_nil; auto.
+  introv isv.
+  destruct isv as [wf cl isc].
+  constructor; eauto 4 with slow.
+  apply iscan_implies in isc.
+  repndors; exrepnd; subst; simpl; auto.
 Qed.
-Hint Resolve implies_isprog_abs2bot : slow.
+Hint Resolve implies_isvalue_abs2bot : slow.
 
-Lemma isnoncan_like_abs2bot {o} :
-  forall (t : @NTerm o),
-    isnoncan_like t -> isnoncan_like (abs2bot t).
+Lemma compute_to_value_abs2bot {o} :
+  forall (t : @NTerm o) u,
+    wf_term t
+    -> computes_to_value [] t u
+    -> {w : NTerm
+        & computes_to_value [] (abs2bot t) w
+        # alpha_eq w (abs2bot u)}.
 Proof.
-  destruct t as [v|f|op bs]; unfold isnoncan_like; simpl; tcsp.
-  intro h.
-  destruct op; tcsp.
+  introv wf comp; allunfold @computes_to_value; repnd.
+  pose proof (reduces_to_abs2bot t u wf comp0) as h; exrepnd.
+  exists w; dands; auto.
+  eapply alpha_preserves_value;[apply alpha_eq_sym;exact h0|].
+  eauto 3 with slow.
 Qed.
-Hint Resolve isnoncan_like_abs2bot : slow.
 
-Lemma eapply_wf_def_sterm {o} :
-  forall (f : @ntseq o),
-    eapply_wf_def (sterm f).
+Lemma lblift_as_combine {o} :
+  forall R (bs1 bs2 : list (@BTerm o)),
+    lblift R bs1 bs2
+    <=> (length bs1 = length bs2
+         # forall b1 b2,
+             LIn (b1,b2) (combine bs1 bs2)
+             -> blift R b1 b2).
 Proof.
   introv.
-  unfold eapply_wf_def; left; eexists; eauto.
+  unfold lblift; split; intro h; repnd; dands; auto; introv i.
+  - apply (in_nth_combine_iff _ _ default_bt default_bt) in i.
+    exrepnd; subst.
+    apply h; auto.
+  - apply h.
+    apply (in_nth_combine_iff _ _ default_bt default_bt).
+    eexists; dands; eauto; auto; try omega.
 Qed.
-Hint Resolve eapply_wf_def_sterm : slow.
 
-Lemma compute_step_abs2bot {o} :
-  forall (t : @NTerm o) u,
-    compute_step [] t = csuccess u
-    -> compute_step [] (abs2bot t) = csuccess (abs2bot u).
+Lemma implies_alpha_eq_abs2bot {o} :
+  forall (t1 t2 : @NTerm o),
+    alpha_eq t1 t2
+    -> alpha_eq (abs2bot t1) (abs2bot t2).
 Proof.
-  nterm_ind1s t as [v|f ind|op bs ind] Case; introv comp.
-
-  - Case "vterm".
-    csunf; allsimpl; ginv.
-
-  - Case "sterm".
-    csunf comp; allsimpl; ginv; auto.
-
-  - Case "oterm".
-    dopid op as [can|ncan|exc|abs] SCase.
-
-    + SCase "Can".
-      csunf comp; allsimpl; ginv; auto.
-
-    + SCase "NCan".
-      destruct bs as [|b1 bs]; try (complete (allsimpl; ginv)).
-      destruct b1 as [l t]; try (complete (allsimpl; ginv)).
-      destruct l; try (complete (allsimpl; ginv)).
-
-      {
-        destruct t as [x|f|op bts]; try (complete (allsimpl; ginv));[|].
-
-        - csunf comp; allsimpl.
-          dopid_noncan ncan SSCase; allsimpl; ginv; auto.
-
-          {
-            SSCase "NApply".
-            apply compute_step_seq_apply_success in comp; exrepnd; subst; allsimpl.
-            csunf; simpl; auto.
-          }
-
-          {
-            SSCase "NEApply".
-
-            apply compute_step_eapply_success in comp; exrepnd; subst.
-            repndors; exrepnd; allsimpl; subst.
-
-            + apply compute_step_eapply2_success in comp1; repnd; subst.
-              repndors; exrepnd; subst; ginv.
-              csunf; simpl.
-              dcwf h; simpl.
-              boolvar; try omega.
-              rewrite Znat.Nat2Z.id; auto.
-
-            + csunf; simpl.
-              apply isexc_implies2 in comp0; exrepnd; subst.
-              dcwf h; simpl; auto.
-
-            + fold_terms.
-              rewrite compute_step_eapply_iscan_isnoncan_like; eauto 3 with slow.
-              pose proof (ind arg2 arg2 []) as h; clear ind.
-              repeat (autodimp h hyp); eauto 3 with slow.
-              apply h in comp1; clear h.
-              rewrite comp1; auto.
-          }
-
-          {
-            SSCase "NFix".
-            apply compute_step_fix_success in comp; repnd; subst.
-            csunf; simpl; auto.
-          }
-
-          {
-            SSCase "NCbv".
-            apply compute_step_cbv_success in comp; exrepnd; subst.
-            csunf; simpl; auto.
-          }
-
-        - dopid op as [can2|ncan2|exc2|abs2] SSCase.
-
-          + SSCase "Can".
-            dopid_noncan ncan SSSCase.
-
-            {
-              SSSCase "NApply".
-
-              csunf comp; allsimpl.
-              apply compute_step_apply_success in comp.
-              repndors; exrepnd; subst; auto.
-            }
-
-            {
-              SSSCase "NEApply".
-
-              csunf comp; allsimpl.
-              apply compute_step_eapply_success in comp.
-              repndors; exrepnd; subst; auto.
-              repndors; exrepnd; subst; allsimpl; auto.
-
-              - apply compute_step_eapply2_success in comp1; repnd; subst.
-                repndors; exrepnd; subst; auto; ginv.
-
-                + unfold mk_lam in *; ginv.
-                  csunf; simpl.
-                  dcwf h; simpl.
-                  apply iscan_implies in comp0; repndors; exrepnd; subst; simpl; auto.
-
-                + unfold mk_nseq in *; allsimpl; ginv.
-                  csunf; simpl.
-                  dcwf h; simpl.
-                  boolvar; simpl; auto; try omega.
-                  rewrite Znat.Nat2Z.id; auto.
-
-              - fold_terms; rewrite compute_step_eapply_iscan_isexc; auto.
-
-              - fold_terms; rewrite compute_step_eapply_iscan_isnoncan_like; auto.
-
-                pose proof (ind arg2 arg2 []) as q; clear ind.
-                repeat (autodimp q hyp); eauto 2 with slow.
-                apply q in comp1; clear q.
-                rewrite comp1; auto.
-            }
-
-            {
-              SSSCase "NFix".
-
-              csunf comp; allsimpl.
-              apply compute_step_fix_success in comp.
-              repndors; exrepnd; subst; auto.
-            }
-
-            {
-              SSSCase "NSpread".
-
-              csunf comp; allsimpl.
-              apply compute_step_spread_success in comp.
-              repndors; exrepnd; subst; auto.
-            }
-
-            {
-              SSSCase "NDsup".
-
-              csunf comp; allsimpl.
-              apply compute_step_dsup_success in comp.
-              repndors; exrepnd; subst; auto.
-            }
-
-            {
-              SSSCase "NDecide".
-
-              csunf comp; allsimpl.
-              apply compute_step_decide_success in comp.
-              repndors; exrepnd; subst; auto.
-              repndors; exrepnd; subst; auto.
-            }
-
-            {
-              SSSCase "NCbv".
-
-              csunf comp; allsimpl.
-              apply compute_step_cbv_success in comp.
-              repndors; exrepnd; subst; auto.
-            }
-
-            {
-              SSSCase "NSleep".
-
-              csunf comp; allsimpl.
-              apply compute_step_sleep_success in comp.
-              repndors; exrepnd; subst; auto.
-            }
-
-            {
-              SSSCase "NTUni".
-
-              csunf comp; allsimpl.
-              apply compute_step_tuni_success in comp.
-              repndors; exrepnd; subst; auto.
-              csunf; simpl.
-              unfold compute_step_tuni; simpl.
-              boolvar; try omega.
-              rewrite Znat.Nat2Z.id; auto.
-            }
-
-            {
-              SSSCase "NMinus".
-
-              csunf comp; allsimpl.
-              apply compute_step_minus_success in comp.
-              repndors; exrepnd; subst; auto.
-            }
-
-            {
-              SSSCase "NFresh".
-
-              csunf comp; allsimpl; ginv.
-            }
-
-            {
-              SSSCase "NTryCatch".
-
-              csunf comp; allsimpl.
-              apply compute_step_try_success in comp.
-              repndors; exrepnd; subst; auto.
-            }
-
-            {
-              SSSCase "NParallel".
-
-              csunf comp; allsimpl.
-              apply compute_step_parallel_success in comp.
-              repndors; exrepnd; subst; auto.
-            }
-
-            {
-              SSSCase "NCompOp".
-
-              apply compute_step_ncompop_can1_success in comp; repnd.
-              repndors; exrepnd; allsimpl; subst; tcsp.
-
-              - csunf; simpl.
-                dcwf h.
-
-              - rewrite compute_step_ncompop_ncanlike2; auto.
-                dcwf h.
-                pose proof (ind t t []) as q; clear ind.
-                repeat (autodimp q hyp); eauto 2 with slow.
-                apply q in comp4; clear q.
-                rewrite comp4; auto.
-
-              - csunf; simpl.
-                apply isexc_implies2 in comp1; exrepnd; subst.
-                dcwf h; simpl; auto.
-            }
-
-            {
-              SSSCase "NArithOp".
-
-              apply compute_step_narithop_can1_success in comp; repnd.
-              repndors; exrepnd; allsimpl; subst; tcsp.
-
-              - csunf; simpl.
-                dcwf h.
-
-              - rewrite compute_step_narithop_ncanlike2; auto.
-                dcwf h.
-                pose proof (ind t t []) as q; clear ind.
-                repeat (autodimp q hyp); eauto 2 with slow.
-                apply q in comp4; clear q.
-                rewrite comp4; auto.
-
-              - csunf; simpl.
-                apply isexc_implies2 in comp1; exrepnd; subst.
-                dcwf h; simpl; auto.
-            }
-
-            {
-              SSSCase "NCanTest".
-
-              csunf comp; allsimpl.
-              apply compute_step_can_test_success in comp.
-              repndors; exrepnd; subst; auto.
-            }
-
-          + SSCase "NCan".
-
-            csunf comp; allsimpl.
-            remember (compute_step lib (oterm (NCan ncan2) bts)) as c.
-            destruct c; allsimpl; ginv.
-            symmetry in Heqc.
-
-            pose proof (ind (oterm (NCan ncan2) bts) (oterm (NCan ncan2) bts) []) as q; clear ind.
-            repeat (autodimp q hyp); eauto 2 with slow.
-            apply q in Heqc; clear q.
-            csunf; simpl.
-            rewrite Heqc; auto.
-
-          + SSCase "Exc".
-
-            csunf comp; allsimpl.
-            apply compute_step_catch_success in comp.
-            repndors; exrepnd; subst; allsimpl; ginv.
-
-            * csunf; simpl; auto.
-
-            * csunf; simpl; auto.
-              rewrite compute_step_catch_if_diff; auto.
-
-          + SSCase "Abs".
-
-            csunf comp; allsimpl.
-            remember (compute_step lib (oterm (Abs abs2) bts)) as c.
-            destruct c; allsimpl; ginv.
-            symmetry in Heqc.
-
-            pose proof (ind (oterm (Abs abs2) bts) (oterm (Abs abs2) bts) []) as q; clear ind.
-            repeat (autodimp q hyp); eauto 2 with slow.
-            apply q in Heqc; clear q.
-            csunf; simpl.
-            rewrite Heqc; auto.
-      }
-
-      {
-        csunf comp; allsimpl.
-        apply compute_step_fresh_success in comp; exrepnd; subst.
-        repndors; exrepnd; subst; ginv.
-
-        - csunf; simpl; boolvar; auto.
-
-        - rewrite compute_step_fresh_if_isvalue_like2; auto.
-
-        - rewrite compute_step_fresh_if_isnoncan_like; auto.
-
-          pose proof (ind t (subst t n (mk_utoken (get_fresh_atom t))) [n]) as q; clear ind.
-          repeat (autodimp q hyp); eauto 2 with slow.
-          { rewrite simple_osize_subst; eauto 2 with slow. }
-          apply q in comp2; clear q.
-          rewrite comp2; simpl; auto.
-      }
-
-    + SCase "Exc".
-
-      csunf comp; allsimpl; ginv.
-
-    + SCase "Abs".
-
-      csunf comp; allsimpl.
-      apply compute_step_lib_success in comp.
-      exrepnd; subst.
-
-      csunf; simpl.
-      destruct e.
-      apply (found_entry_implies_compute_step_lib_success _ _ _ _ _ _ correct).
-
-      apply found_entry_add_new_abs; auto.
+  introv aeq.
+  allrw @abs2bot_as_abs2vbot; eauto 3 with slow.
 Qed.
+Hint Resolve implies_alpha_eq_abs2bot : slow.
 
 Lemma approx_nil_abs2bot_1 {o} :
   forall (t : @NTerm o), isprog t -> approx [] t (abs2bot t).
 Proof.
-  cofix CIH.
+  unfold approx.
+  pose proof (@approx_acc_resp o [] (fun x y => isprog x # alpha_eq y (abs2bot x))) as HH.
+  allsimpl.
 
-  introv isp.
+  assert (forall x y : @NTerm o, (isprog x # alpha_eq y (abs2bot x)) -> approx_aux [] bot2 x y);[|tcsp];[].
+  apply HH; eauto 3 with slow;
+  try (complete (introv aeq h; allsimpl; repnd; subst; dands; eauto 3 with slow)).
+
+  introv hr1 hr2 resp1 resp2 aeq; repnd.
+  rename x1 into u.
+  rename x0 into t.
+
+  eapply respects_alpha_r_approx_aux;[|apply alpha_eq_sym;exact aeq|]; auto.
+  clear dependent u.
+
   constructor.
-  unfold close_comput; dands; eauto 3 with slow;
+  unfold close_comput; dands; eauto 3 with slow.
   introv comp.
 
-  - SearchAbout abs2bot.
+  - applydup @compute_to_value_abs2bot in comp; eauto 3 with slow.
+    exrepnd.
+    allsimpl.
+    apply alpha_eq_sym in comp1; apply alpha_eq_oterm_implies_combine in comp1.
+    exrepnd; subst; allsimpl.
+    rewrite map_length in *.
+    eexists; dands;[exact comp0|].
 
+    apply lblift_as_combine; dands; auto.
+    introv i.
+    pose proof (comp2 (abs2bot_bterm b1) b2) as h.
+    autodimp h hyp.
+    {
+      rewrite <- map_combine_left.
+      apply in_map_iff.
+      exists (b1,b2); simpl; dands; auto.
+    }
+
+    eapply blift_alpha_fun_r;[|exact h].
+    apply in_combine in i; repnd.
+
+    unfold computes_to_value in comp; repnd.
+    inversion comp as [? isp isc]; subst; clear comp.
+    apply isprogram_eq in isp.
+    apply isprog_ot_iff in isp; repnd.
+    applydup isp in i0.
+
+    clear dependent b2.
+    destruct b1 as [l u]; allsimpl.
+    apply isprogram_bt_eq in i1.
+    apply isprogam_bt_nt_wf_eauto in i1.
+
+    unfold blift.
+    exists l u (abs2bot u).
+    dands; auto.
+
+    apply approx_open_simpler_equiv_r; eauto 3 with slow.
+    unfold simpl_olift; dands; eauto 3 with slow.
+    introv ps isp1 isp2.
+
+    right.
+
+    (* It should be allowed to only replace some abstractions by bottom! *)
+
+  -
+
+  -
 Qed.
 
 Lemma approx_nil_abs2bot_1 {o} :
@@ -1700,31 +1352,7 @@ Proof.
         apply isprog_vars_isprogrambt in i0.
         unfold simpl_olift; dands; eauto 3 with slow.
 
-        {
-          pose proof (implies_props_abs2bot t) as h; repnd.
-          eauto 3 with slow.
-        }
-
         introv ps isp1 isp2.
-        repeat (rw @cl_lsubst_lsubst_aux; eauto 2 with slow); simpl.
-
-
-Lemma lsubst_aux_abs2bot {o} :
-  forall (t : @NTerm o) sub,
-    lsubst_aux (abs2bot t) sub = abs2bot (lsubst_aux t sub).
-Proof.
-  nterm_ind t as [v|f ind|op bs ind] Case; introv; simpl; auto.
-
-  - Case "vterm".
-    remember (sub_find sub v) as sf; symmetry in Heqsf; destruct sf; simpl; auto.
-Qed.
-
-
-        rw @cl_lsubst_lsubst_aux; eauto 2 with slow.
-        pose proof (ind t t l i1) as h; clear ind.
-        repeat (autodimp h hyp); eauto 3 with slow.
-
-        SearchAbout blift_sub.
 Qed.
 
 Lemma cequiv_nil_abs2bot {o} :
