per/per_props_nat.v
@@ -2,6 +2,7 @@
 
   Copyright 2014 Cornell University
   Copyright 2015 Cornell University
+  Copyright 2016 Cornell University
 
   This file is part of VPrl (the Verified Nuprl project).
 
@@ -16,15 +17,18 @@
   GNU General Public License for more details.
 
   You should have received a copy of the GNU General Public License
-  along with VPrl.  Ifnot, see <http://www.gnu.org/licenses/>.
+  along with VPrl.  If not, see <http://www.gnu.org/licenses/>.
 
 
-  Website: http://nuprl.org/html/verification/
+  Website : http://nuprl.org/html/verification/
+            http://nuprl.org/html/Nuprl2Coq
+            https://github.com/vrahli/NuprlInCoq
+
   Authors: Abhishek Anand & Vincent Rahli
 
 *)
 
-Require Export alphaeq3.
+Require Export alphaeq5.
 Require Export cvterm.
 Require Export nat_defs.
 Require Export per_props_set.
@@ -1123,26 +1127,6 @@ Lemma ite_same :
     (if b then x else x) = x.
 Proof.
   introv; destruct b; tcsp.
-Qed.
-
-Lemma alpha_eq_bterm_bterm_disjoint {o} :
-  forall vs1 vs2 (t : @NTerm o),
-    disjoint vs1 (free_vars t)
-    -> disjoint vs2 (free_vars t)
-    -> length vs1 = length vs2
-    -> alpha_eq_bterm (bterm vs1 t) (bterm vs2 t).
-Proof.
-  introv d1 d2 len.
-  pose proof (fresh_vars (length vs1)
-                         (vs1 ++ vs2
-                              ++ free_vars t
-                              ++ bound_vars t)) as fvs; exrepnd.
-  allrw disjoint_app_r; repnd.
-  apply (al_bterm_aux lvn); auto.
-  { allrw disjoint_app_r; tcsp. }
-  rw @lsubst_aux_trivial_cl_term;[|rw @dom_sub_var_ren;eauto with slow].
-  rw @lsubst_aux_trivial_cl_term;[|rw @dom_sub_var_ren;eauto with slow; try omega].
-  eauto with slow.
 Qed.
 
 Lemma mkcv_natk_substc {o} :
